src/RatUtil.v
@@ -1,0 +1,20 @@
+Require Import FCF.
+Require Import Coq.Classes.Morphisms.
+
+Create HintDb rat discriminated.
+Create HintDb ratsimpl discriminated.
+
+Hint Immediate (@reflexivity Rat eqRat _) : rat.
+Hint Immediate (@reflexivity Rat leRat _) : rat.
+
+Lemma maxRat_same r : maxRat r r = r.
+Proof. intros; cbv [maxRat]; destruct (bleRat r r) eqn:?; trivial. Qed.
+Lemma minRat_same r : minRat r r = r.
+Proof. intros; cbv [minRat]; destruct (bleRat r r) eqn:?; trivial. Qed.
+
+Hint Rewrite ratSubtract_0 minRat_same maxRat_same : ratsimpl.
+
+Lemma ratDistance_same r : ratDistance r r == 0.
+Proof. cbv [ratDistance]; autorewrite with ratsimpl; auto with rat. Qed.
+
+Hint Rewrite ratDistance_same : ratsimpl.
