src/RewriteUtil.v
@@ -1,0 +1,108 @@
+Require Import FCF.
+Require Import Asymptotic.
+Require Import RatUtil.
+Require Import Coq.Lists.SetoidList.
+
+Global Instance Proper_negligible :
+  Proper (pointwise_relation nat eqRat ==> iff) negligible.
+Proof.
+  cbv [pointwise_relation Proper respectful].
+  split; eauto 10 using negligible_eq, (@symmetry _ eqRat _).
+Qed.
+
+Global Instance Proper_negligible_le :
+  Proper (pointwise_relation nat leRat ==> Basics.flip Basics.impl) negligible.
+Proof.
+  cbv [pointwise_relation Proper respectful].
+  intros ? ? ? ?; eauto using negligible_le.
+Qed.
+
+Lemma negligible_0 : negligible (fun _ => 0).
+  eapply negligible_le with (f1 := fun n => 0 / expnat 2 n).
+  { reflexivity. }
+  { apply negligible_const_num. }
+Qed.
+
+Definition image_relation {T} (R:T->T->Prop) {A} (f:A->T) := fun x y => R (f x) (f y).
+Global Instance Equivalence_image_relation {T R} {Equivalence_R:Equivalence R} {A} (f:A->T) :
+  Equivalence (image_relation R f).
+Proof. destruct Equivalence_R; split; cbv; eauto. Qed.
+Definition Distribution_eq {A} := pointwise_relation A eqRat.
+
+Global Instance Equivalence_Distribution_eq {A} : Equivalence (@Distribution_eq A).
+Proof.
+  split; repeat intro; eauto using (@symmetry _ eqRat _), (@transitivity _ eqRat _) with rat.
+Qed.
+
+Definition Comp_eq {A} := image_relation Distribution_eq (@evalDist A).
+Global Instance Equivalence_Comp_eq {A} : Equivalence (@Comp_eq A) := _.
+
+Global Instance Proper_evalDist {A} : Proper (Comp_eq ==> Distribution_eq) (@evalDist A).
+Proof. exact (fun _ _ => id). Qed.
+
+Global Instance Proper_getSupport {A} : Proper (Comp_eq ==> (@Permutation.Permutation _)) (@getSupport A).
+Proof. intros ???; eapply evalDist_getSupport_perm_id; assumption. Qed.
+
+Global Instance Proper_sumList {A:Set} {R:A->A->Prop} : Proper (eqlistA R  ==> (R ==> eqRat) ==> eqRat) (@sumList A).
+Proof.
+  repeat intro. cbv [sumList].
+  rewrite <-!fold_left_rev_right.
+  eapply eqlistA_rev in H.
+  generalize dependent (rev x); generalize dependent (rev y).
+  intros ? ?; induction 1; [reflexivity|].
+  simpl; f_equiv; eauto.
+Qed.
+
+Global Instance Proper_sumList_permutation {A:Set} : Proper ((@Permutation.Permutation A) ==> (Logic.eq ==> eqRat) ==> eqRat) (@sumList A).
+Proof.
+  intros ? ? H; induction H; repeat intro; cbv [respectful] in *; rewrite ?sumList_cons.
+  { eauto with rat. }
+  { f_equiv; eauto. }
+  { repeat rewrite H by reflexivity.
+    repeat rewrite <-ratAdd_assoc.
+    rewrite (ratAdd_comm (y0 y)).
+    f_equiv.
+    eapply (Proper_sumList(R:=Logic.eq)); eauto; reflexivity. }
+  { etransitivity; [eapply IHPermutation1 | eapply IHPermutation2];
+      intros; subst; (try match goal with H1:_ |- _ => eapply H1 end;reflexivity). }
+Qed.
+
+Global Instance Proper_Bind {A B} : Proper (Comp_eq ==> (Logic.eq==>Comp_eq) ==> Comp_eq) (@Bind A B).
+Proof.
+  intros ?? H ?? G ?. simpl evalDist.
+
+  (* TODO: find out why setoid rewrite does not do this *)
+  etransitivity; [|reflexivity].
+  eapply Proper_sumList_permutation.
+  eapply Proper_getSupport.
+  eassumption.
+  intros ? ? ?; subst.
+  f_equiv.
+  { eapply Proper_evalDist. assumption. }
+  { eapply Proper_evalDist. eapply G. reflexivity. }
+Qed.
+
+Lemma eq_impl_negligible : forall A (x y : nat -> Comp A), pointwise_relation _ Comp_eq x y -> forall t, negligible (fun eta : nat => | evalDist (x eta) t - evalDist (y eta) t|).
+Admitted.
+
+Lemma Comp_eq_bool (x y:Comp bool) :
+  well_formed_comp x
+  -> well_formed_comp y
+  -> Pr [x] == Pr[y]
+  -> Comp_eq x y.
+  intros.
+  intro b.
+  destruct b; trivial.
+  rewrite !evalDist_complement; trivial.
+  f_equiv; trivial.
+Qed.
+
+Lemma Comp_eq_evalDist A (x y:Comp A) :
+  well_formed_comp x
+  -> well_formed_comp y
+  -> (forall c, evalDist x c == evalDist y c)
+  -> Comp_eq x y.
+  intros.
+  intro b.
+  apply H1.
+Qed.
