src/Util.v
@@ -1,0 +1,20 @@
+Require Import FCF.
+Require Import SplitVector.
+Require Import RewriteUtil.
+
+Lemma Rnd_split_eq n1 n2 : Comp_eq
+                                (x <-$ { 0 , 1 }^ n1 + n2; ret splitVector n1 n2 x)
+                                (x1 <-$ { 0 , 1 }^ n1; x2 <-$ { 0 , 1 }^ n2; ret (x1, x2)).
+Proof. intro z. eapply Rnd_split_equiv. Qed.
+
+Lemma list_vector_split a b (T : Set) (x : Vector.t T _) : skipn (b) (Vector.to_list x) = Vector.to_list (snd (splitVector (b) a x)).
+  induction b; simpl; intuition.
+  destruct (splitVector b a (Vector.tl x)) eqn:?.
+  specialize (IHb (Vector.tl x)).
+  rewrite Heqp in IHb.
+  simpl in *.
+  rewrite <- IHb.
+  SearchAbout Vector.hd Vector.tl.
+  rewrite (Vector.eta x).
+  reflexivity.
+Qed.
